code/ecdsa/Hacl.Impl.SolinasReduction.P256.fst
@@ -22,7 +22,7 @@ open FStar.Mul
 module BV = FStar.BitVector
 module Seq = FStar.Seq
 
-
+#set-options "--fuel 0 --ifuel 0 --z3rlimit 100"
 
 inline_for_extraction noextract
 val get_high_part: a:uint64 -> r:uint32{uint_v r == uint_v a / pow2 32}
@@ -105,16 +105,17 @@ let store_high_low_u high low =
   lemma_xor_zero as_uint64_low as_uint64_high;
   logxor as_uint64_low as_uint64_high
 
-#push-options "--z3rlimit 100"
+
+#push-options "--z3rlimit 100 --fuel 1"
+
 
 inline_for_extraction noextract
 val load_buffer: a0: uint64 -> a1: uint64 -> a2: uint64 -> a3: uint64
   -> o: lbuffer uint64 (size 4)
   -> Stack unit
-    (requires fun h -> live h o)
-    (ensures  fun h0 _ h1 ->
-       modifies (loc o) h0 h1 /\
-       as_nat P256 h1 o = v a0 + v a1 * pow2 64 + v a2 * pow2 128 + v a3 * pow2 192)
+  (requires fun h -> live h o)
+  (ensures  fun h0 _ h1 -> modifies (loc o) h0 h1 /\
+    as_nat P256 h1 o = v a0 + v a1 * pow2 64 + v a2 * pow2 128 + v a3 * pow2 192)
 
 let load_buffer a0 a1 a2 a3 o =
   assert_norm (pow2 64 * pow2 64 = pow2 128);
@@ -122,118 +123,124 @@ let load_buffer a0 a1 a2 a3 o =
   upd o (size 0) a0;
   upd o (size 1) a1;
   upd o (size 2) a2;
-  upd o (size 3) a3
+  upd o (size 3) a3;
+
+  let h0 = ST.get() in 
+
+  let o_seq = as_seq h0 o in 
+  lseq_as_nat_definiton o_seq 0;
+  lseq_as_nat_definiton o_seq 1;
+  lseq_as_nat_definiton o_seq 2;
+  lseq_as_nat_definiton o_seq 3
+
+#pop-options
+
 
 inline_for_extraction noextract
-val upl_zer_buffer:
-    c0: uint32 -> c1: uint32 -> c2: uint32 -> c3: uint32
-  -> c4: uint32 -> c5: uint32 -> c6: uint32 -> c7: uint32
-  -> o: lbuffer uint64 (size 4) ->
+val upl_zer_buffer: c0: uint32 -> c1: uint32 -> c2: uint32 -> c3: uint32 -> c4: uint32 -> c5: uint32 -> c6: uint32 
+  -> c7: uint32 -> o: lbuffer uint64 (size 4) ->
   Stack unit
-    (requires fun h -> live h o)
-    (ensures fun h0 _ h1 ->
-      modifies (loc o) h0 h1 /\
-      as_nat P256 h1 o == (v c0 + v c1 * pow2 (1 * 32) + v c2 * pow2 (2 * 32) + v c3 * pow2 (3 * 32) + v c4 * pow2 (4 * 32) + v c5 * pow2 (5 * 32) + v  c6 * pow2 (6 * 32) + v c7 * pow2 (7 * 32)) % prime256
-   )
+  (requires fun h -> live h o)
+  (ensures fun h0 _ h1 -> modifies (loc o) h0 h1 /\
+    as_nat P256 h1 o == (v c0 + v c1 * pow2 (1 * 32) + v c2 * pow2 (2 * 32) + v c3 * pow2 (3 * 32) + v c4 * pow2 (4 * 32) + v c5 * pow2 (5 * 32) + v  c6 * pow2 (6 * 32) + v c7 * pow2 (7 * 32)) % prime256)
 
 let upl_zer_buffer c0 c1 c2 c3 c4 c5 c6 c7 o =
-    let b0 = store_high_low_u c1 c0 in
-    let b1 = store_high_low_u c3 c2 in
-    let b2 = store_high_low_u c5 c4 in
-    let b3 = store_high_low_u c7 c6 in
+  let b0 = store_high_low_u c1 c0 in
+  let b1 = store_high_low_u c3 c2 in
+  let b2 = store_high_low_u c5 c4 in
+  let b3 = store_high_low_u c7 c6 in
     assert_norm (pow2 (1 * 32) * pow2 (2 * 32) = pow2 (3 * 32));
     assert_norm (pow2 (2 * 32) * pow2 (2 * 32) = pow2 (4 * 32));
     assert_norm (pow2 (3 * 32) * pow2 (2 * 32) = pow2 (5 * 32));
     assert_norm (pow2 (4 * 32) * pow2 (2 * 32) = pow2 (6 * 32));
     assert_norm (pow2 (5 * 32) * pow2 (2 * 32) = pow2 (7 * 32));
 
-    assert(v b0 = v c1 * pow2 32 + v c0);
-    assert(v b1 = v c3 * pow2 32 + v c2);
-    assert(v b2 = v c5 * pow2 32 + v c4);
-    assert(v b3 = v c7 * pow2 32 + v c6);
-
-    load_buffer b0 b1 b2 b3 o;
-    reduction_prime_2prime #P256 o o;
-    let h2 = ST.get() in
-    assert(as_nat P256 h2 o = (v c1 * pow2 32 + v c0 + v c3 * pow2 (3 * 32) + v c2 * pow2 (2 * 32) + v c5 * pow2 (32 * 5) + v c4 * pow2 (32 * 4) + v c7 * pow2 (32 * 7) + v c6 * pow2 (32 * 6)) % prime256)
+  load_buffer b0 b1 b2 b3 o;
+  reduction_prime_2prime #P256 o o
 
 
 inline_for_extraction noextract
 val upl_fir_buffer: c11: uint32 -> c12: uint32 -> c13: uint32 -> c14: uint32 -> c15: uint32
   -> o: lbuffer uint64 (size 4) ->
   Stack unit
-    (requires fun h -> live h o)
-    (ensures fun h0 _ h1 ->
-      modifies (loc o) h0 h1 /\
-      as_nat P256 h1 o == (v c11 * pow2 (3 * 32) + v c12 * pow2 (4 * 32) + v c13 * pow2 (5 * 32) + v c14 * pow2 (6 * 32) + v c15 * pow2 (7 * 32)) % prime256
-    )
+  (requires fun h -> live h o)
+  (ensures fun h0 _ h1 -> modifies (loc o) h0 h1 /\
+    as_nat P256 h1 o == (v c11 * pow2 (3 * 32) + v c12 * pow2 (4 * 32) + v c13 * pow2 (5 * 32) + v c14 * pow2 (6 * 32) + v c15 * pow2 (7 * 32)) % prime256)
 
 let upl_fir_buffer c11 c12 c13 c14 c15 o =
-      assert_norm (pow2 (1 * 32) * pow2 (2 * 32) = pow2 (3 * 32));
-      assert_norm (pow2 (2 * 32) * pow2 (2 * 32) = pow2 (4 * 32));
-      assert_norm (pow2 (3 * 32) * pow2 (2 * 32) = pow2 (5 * 32));
-      assert_norm (pow2 (4 * 32) * pow2 (2 * 32) = pow2 (6 * 32));
-      assert_norm (pow2 (5 * 32) * pow2 (2 * 32) = pow2 (7 * 32));
-  let b0 = u64(0) in
+  assert_norm (pow2 (1 * 32) * pow2 (2 * 32) = pow2 (3 * 32));
+  assert_norm (pow2 (2 * 32) * pow2 (2 * 32) = pow2 (4 * 32));
+  assert_norm (pow2 (3 * 32) * pow2 (2 * 32) = pow2 (5 * 32));
+  assert_norm (pow2 (4 * 32) * pow2 (2 * 32) = pow2 (6 * 32));
+  assert_norm (pow2 (5 * 32) * pow2 (2 * 32) = pow2 (7 * 32));
+  
+  let b0 = u64 0 in
   let b1 = store_high_low_u c11 (u32 0) in
   let b2 = store_high_low_u c13 c12 in
   let b3 = store_high_low_u c15 c14 in
+  
   load_buffer b0 b1 b2 b3 o;
   reduction_prime_2prime #P256 o o
+
 
 inline_for_extraction noextract
 val upl_sec_buffer: c12: uint32 -> c13: uint32 -> c14: uint32 -> c15: uint32
   -> o: lbuffer uint64 (size 4) ->
   Stack unit
-    (requires fun h -> live h o)
-    (ensures fun h0 _ h1 ->
-      modifies (loc o) h0 h1 /\
-      as_nat P256 h1 o == (v c12 * pow2 (3 * 32) + v c13 * pow2 (4 * 32) + v c14 * pow2 (5 * 32) + v c15 * pow2 (6 * 32)) % prime /\ as_nat P256 h1 o < prime
-    )
+  (requires fun h -> live h o)
+  (ensures fun h0 _ h1 -> modifies (loc o) h0 h1 /\ as_nat P256 h1 o < prime /\
+    as_nat P256 h1 o == (v c12 * pow2 (3 * 32) + v c13 * pow2 (4 * 32) + v c14 * pow2 (5 * 32) + v c15 * pow2 (6 * 32)) % prime
+  )
 
 let upl_sec_buffer c12 c13 c14 c15 o =
-      assert_norm (pow2 (1 * 32) * pow2 (2 * 32) = pow2 (3 * 32));
-      assert_norm (pow2 (2 * 32) * pow2 (2 * 32) = pow2 (4 * 32));
-      assert_norm (pow2 (3 * 32) * pow2 (2 * 32) = pow2 (5 * 32));
-      assert_norm (pow2 (4 * 32) * pow2 (2 * 32) = pow2 (6 * 32));
-      assert_norm (pow2 (5 * 32) * pow2 (2 * 32) = pow2 (7 * 32));
-    let b0 = u64 (0) in
-    let b1 = store_high_low_u c12 (u32 0) in
-    let b2 = store_high_low_u c14 c13 in
-    let b3 = store_high_low_u (u32 0) c15 in
-    load_buffer b0 b1 b2 b3 o;
-    assert_norm(v c12 * pow2 (3 * 32) + v c13 * pow2 (4 * 32) + v c14 * pow2 (5 * 32) + v c15 * pow2 (6 * 32) < prime);
-    let h1 = ST.get() in
-    modulo_lemma (as_nat P256 h1 o) prime
+  assert_norm (pow2 (1 * 32) * pow2 (2 * 32) = pow2 (3 * 32));
+  assert_norm (pow2 (2 * 32) * pow2 (2 * 32) = pow2 (4 * 32));
+  assert_norm (pow2 (3 * 32) * pow2 (2 * 32) = pow2 (5 * 32));
+  assert_norm (pow2 (4 * 32) * pow2 (2 * 32) = pow2 (6 * 32));
+  assert_norm (pow2 (5 * 32) * pow2 (2 * 32) = pow2 (7 * 32));
+  
+  let b0 = u64 0 in
+  let b1 = store_high_low_u c12 (u32 0) in
+  let b2 = store_high_low_u c14 c13 in
+  let b3 = store_high_low_u (u32 0) c15 in
+  load_buffer b0 b1 b2 b3 o;
+  assert_norm(v c12 * pow2 (3 * 32) + v c13 * pow2 (4 * 32) + v c14 * pow2 (5 * 32) + v c15 * pow2 (6 * 32) < prime);
+  
+  let h1 = ST.get() in
+  modulo_lemma (as_nat P256 h1 o) prime
+
 
 inline_for_extraction noextract
 val upl_thi_buffer: c8: uint32 -> c9: uint32 -> c10: uint32 -> c14: uint32 -> c15: uint32
   -> o: lbuffer uint64 (size 4) ->
   Stack unit
- (requires fun h -> live h o)
- (ensures fun h0 _ h1 -> modifies (loc o) h0 h1 /\
-      as_nat P256 h1 o == (v c8 + v c9 * pow2 32 + v c10 * pow2 (2 * 32) +  v c14 * pow2 (6 * 32) + v c15 * pow2 (7 * 32)) % prime256)
+  (requires fun h -> live h o)
+  (ensures fun h0 _ h1 -> modifies (loc o) h0 h1 /\
+    as_nat P256 h1 o == (v c8 + v c9 * pow2 32 + v c10 * pow2 (2 * 32) +  v c14 * pow2 (6 * 32) + v c15 * pow2 (7 * 32)) % prime256)
 
 let upl_thi_buffer c8 c9 c10 c14 c15 o =
-   assert_norm (pow2 (1 * 32) * pow2 (2 * 32) = pow2 (3 * 32));
-   assert_norm (pow2 (2 * 32) * pow2 (2 * 32) = pow2 (4 * 32));
-   assert_norm (pow2 (3 * 32) * pow2 (2 * 32) = pow2 (5 * 32));
-   assert_norm (pow2 (4 * 32) * pow2 (2 * 32) = pow2 (6 * 32));
-   assert_norm (pow2 (5 * 32) * pow2 (2 * 32) = pow2 (7 * 32));
-   let b0 = store_high_low_u c9 c8 in
-   let b1 = store_high_low_u (u32 0) c10 in
-   let b2 = u64 0 in
-   let b3 = store_high_low_u c15 c14 in
-   load_buffer b0 b1 b2 b3 o;
-   reduction_prime_2prime #P256 o o
+  assert_norm (pow2 (1 * 32) * pow2 (2 * 32) = pow2 (3 * 32));
+  assert_norm (pow2 (2 * 32) * pow2 (2 * 32) = pow2 (4 * 32));
+  assert_norm (pow2 (3 * 32) * pow2 (2 * 32) = pow2 (5 * 32));
+  assert_norm (pow2 (4 * 32) * pow2 (2 * 32) = pow2 (6 * 32));
+  assert_norm (pow2 (5 * 32) * pow2 (2 * 32) = pow2 (7 * 32));
+   
+  let b0 = store_high_low_u c9 c8 in
+  let b1 = store_high_low_u (u32 0) c10 in
+  let b2 = u64 0 in
+  let b3 = store_high_low_u c15 c14 in
+  
+  load_buffer b0 b1 b2 b3 o;
+  reduction_prime_2prime #P256 o o
+
 
 inline_for_extraction noextract
-val upl_for_buffer: c8: uint32 -> c9: uint32 -> c10: uint32 -> c11: uint32 -> c13: uint32 ->
-  c14: uint32 -> c15: uint32-> o: lbuffer uint64 (size 4) ->
+val upl_for_buffer: c8: uint32 -> c9: uint32 -> c10: uint32 -> c11: uint32 -> c13: uint32 -> c14: uint32 -> c15: uint32 
+  -> o: lbuffer uint64 (size 4) ->
   Stack unit
-    (requires fun h -> live h o)
-    (ensures fun h0 _ h1 -> modifies (loc o) h0 h1 /\
-        as_nat P256 h1 o == (v c9 + v c10 * pow2 32 + v c11 * pow2 (2 * 32) + v c13 * pow2 (3 * 32) + v c14 * pow2 (4 * 32) + v c15 * pow2 (5 * 32) + v c13 * pow2 (6 * 32) +  v c8 * pow2 (7 * 32)) % prime256)
+  (requires fun h -> live h o)
+  (ensures fun h0 _ h1 -> modifies (loc o) h0 h1 /\
+    as_nat P256 h1 o == (v c9 + v c10 * pow2 32 + v c11 * pow2 (2 * 32) + v c13 * pow2 (3 * 32) + v c14 * pow2 (4 * 32) + v c15 * pow2 (5 * 32) + v c13 * pow2 (6 * 32) +  v c8 * pow2 (7 * 32)) % prime256)
 
 let upl_for_buffer c8 c9 c10 c11 c13 c14 c15 o =
   assert_norm (pow2 (1 * 32) * pow2 (2 * 32) = pow2 (3 * 32));
@@ -241,42 +248,47 @@ let upl_for_buffer c8 c9 c10 c11 c13 c14 c15 o =
   assert_norm (pow2 (3 * 32) * pow2 (2 * 32) = pow2 (5 * 32));
   assert_norm (pow2 (4 * 32) * pow2 (2 * 32) = pow2 (6 * 32));
   assert_norm (pow2 (5 * 32) * pow2 (2 * 32) = pow2 (7 * 32));
+  
   let b0 = store_high_low_u c10 c9 in
   let b1 = store_high_low_u c13 c11 in
   let b2 = store_high_low_u c15 c14 in
   let b3 = store_high_low_u c8 c13 in
+  
   load_buffer b0 b1 b2 b3 o;
   reduction_prime_2prime #P256 o o
+
 
 inline_for_extraction noextract
 val upl_fif_buffer: c8: uint32 -> c10: uint32 -> c11: uint32 -> c12: uint32 -> c13: uint32
   -> o: lbuffer uint64 (size 4) ->
   Stack unit
-    (requires fun h -> live h o)
-    (ensures fun h0 _ h1 -> modifies (loc o) h0 h1 /\
+  (requires fun h -> live h o)
+  (ensures fun h0 _ h1 -> modifies (loc o) h0 h1 /\
     as_nat P256 h1 o == (v c11 + v c12 * pow2 32 + v c13 * pow2 (2 * 32) + v c8 * pow2 (6 * 32) + v c10 * pow2 (7 * 32)) % prime256)
 
 let upl_fif_buffer c8 c10 c11 c12 c13 o =
-     assert_norm (pow2 (1 * 32) * pow2 (2 * 32) = pow2 (3 * 32));
-     assert_norm (pow2 (2 * 32) * pow2 (2 * 32) = pow2 (4 * 32));
-     assert_norm (pow2 (3 * 32) * pow2 (2 * 32) = pow2 (5 * 32));
-     assert_norm (pow2 (4 * 32) * pow2 (2 * 32) = pow2 (6 * 32));
-     assert_norm (pow2 (5 * 32) * pow2 (2 * 32) = pow2 (7 * 32));
-    let b0 = store_high_low_u c12 c11 in
-    let b1 = store_high_low_u (u32 0) c13 in
-    let b2 = u64 0 in
-    let b3 = store_high_low_u c10 c8 in
-    load_buffer b0 b1 b2 b3 o;
-    reduction_prime_2prime #P256 o o
+  assert_norm (pow2 (1 * 32) * pow2 (2 * 32) = pow2 (3 * 32));
+  assert_norm (pow2 (2 * 32) * pow2 (2 * 32) = pow2 (4 * 32));
+  assert_norm (pow2 (3 * 32) * pow2 (2 * 32) = pow2 (5 * 32));
+  assert_norm (pow2 (4 * 32) * pow2 (2 * 32) = pow2 (6 * 32));
+  assert_norm (pow2 (5 * 32) * pow2 (2 * 32) = pow2 (7 * 32));
+  
+  let b0 = store_high_low_u c12 c11 in
+  let b1 = store_high_low_u (u32 0) c13 in
+  let b2 = u64 0 in
+  let b3 = store_high_low_u c10 c8 in
+  
+  load_buffer b0 b1 b2 b3 o;
+  reduction_prime_2prime #P256 o o
+
 
 inline_for_extraction noextract
-val upl_six_buffer: c9: uint32 -> c11: uint32 -> c12: uint32 -> c13: uint32 -> c14: uint32 -> c15: uint32-> 
-  o: lbuffer uint64 (size 4) ->
+val upl_six_buffer: c9: uint32 -> c11: uint32 -> c12: uint32 -> c13: uint32 -> c14: uint32 -> c15: uint32 
+  -> o: lbuffer uint64 (size 4) ->
   Stack unit
-    (requires fun h -> live h o)
-    (ensures fun h0 _ h1 -> modifies (loc o) h0 h1 /\ as_nat P256 h1 o == (
-    v c12 + v c13 * pow2 32 + v c14 * pow2 (2 * 32) + v c15 * pow2 (3 * 32) +
-          v c9 * pow2 (6 * 32) + v c11 * pow2 (7 * 32)) % prime256)
+  (requires fun h -> live h o)
+  (ensures fun h0 _ h1 -> modifies (loc o) h0 h1 /\ 
+    as_nat P256 h1 o == (v c12 + v c13 * pow2 32 + v c14 * pow2 (2 * 32) + v c15 * pow2 (3 * 32) + v c9 * pow2 (6 * 32) + v c11 * pow2 (7 * 32)) % prime256)
 
 let upl_six_buffer c9 c11 c12 c13 c14 c15 o =
   assert_norm (pow2 (1 * 32) * pow2 (2 * 32) = pow2 (3 * 32));
@@ -284,21 +296,23 @@ let upl_six_buffer c9 c11 c12 c13 c14 c15 o =
   assert_norm (pow2 (3 * 32) * pow2 (2 * 32) = pow2 (5 * 32));
   assert_norm (pow2 (4 * 32) * pow2 (2 * 32) = pow2 (6 * 32));
   assert_norm (pow2 (5 * 32) * pow2 (2 * 32) = pow2 (7 * 32));
-    let b0 = store_high_low_u c13 c12 in
-    let b1 = store_high_low_u c15 c14 in
-    let b2 = u64 0 in
-    let b3 = store_high_low_u c11 c9 in
-    load_buffer b0 b1 b2 b3 o;
-    reduction_prime_2prime #P256 o o
+  
+  let b0 = store_high_low_u c13 c12 in
+  let b1 = store_high_low_u c15 c14 in
+  let b2 = u64 0 in
+  let b3 = store_high_low_u c11 c9 in
+  
+  load_buffer b0 b1 b2 b3 o;
+  reduction_prime_2prime #P256 o o
+
 
 inline_for_extraction noextract
 val upl_sev_buffer: c8: uint32 -> c9: uint32 -> c10: uint32 -> c12: uint32 -> c13: uint32 ->
-  c14: uint32 -> c15: uint32
-  -> o: lbuffer uint64 (size 4) ->
+  c14: uint32 -> c15: uint32 -> o: lbuffer uint64 (size 4) ->
   Stack unit
-    (requires fun h -> live h o)
-      (ensures fun h0 _ h1 -> modifies (loc o)  h0 h1 /\
-        as_nat P256 h1 o == (v c13 + v c14 * pow2 32 + v c15 * pow2 (2 * 32) + v c8 * pow2 (3 * 32) +  v c9 * pow2 (4 * 32) + v c10 * pow2 (5 * 32) + v c12 * pow2 (7 * 32)) % prime256)
+  (requires fun h -> live h o)
+  (ensures fun h0 _ h1 -> modifies (loc o)  h0 h1 /\
+    as_nat P256 h1 o == (v c13 + v c14 * pow2 32 + v c15 * pow2 (2 * 32) + v c8 * pow2 (3 * 32) +  v c9 * pow2 (4 * 32) + v c10 * pow2 (5 * 32) + v c12 * pow2 (7 * 32)) % prime256)
 
 let upl_sev_buffer c8 c9 c10 c12 c13 c14 c15 o =
   assert_norm (pow2 (1 * 32) * pow2 (2 * 32) = pow2 (3 * 32));
@@ -306,20 +320,22 @@ let upl_sev_buffer c8 c9 c10 c12 c13 c14 c15 o =
   assert_norm (pow2 (3 * 32) * pow2 (2 * 32) = pow2 (5 * 32));
   assert_norm (pow2 (4 * 32) * pow2 (2 * 32) = pow2 (6 * 32));
   assert_norm (pow2 (5 * 32) * pow2 (2 * 32) = pow2 (7 * 32));
-    let b0 = store_high_low_u c14 c13 in
-    let b1 = store_high_low_u c8 c15 in
-    let b2 = store_high_low_u c10 c9 in
-    let b3 = store_high_low_u c12 (u32 0) in
-    load_buffer b0 b1 b2 b3 o;
-    reduction_prime_2prime #P256 o o
+  
+  let b0 = store_high_low_u c14 c13 in
+  let b1 = store_high_low_u c8 c15 in
+  let b2 = store_high_low_u c10 c9 in
+  let b3 = store_high_low_u c12 (u32 0) in
+  
+  load_buffer b0 b1 b2 b3 o;
+  reduction_prime_2prime #P256 o o
+
 
 inline_for_extraction noextract
 val upl_eig_buffer: c9: uint32 -> c10: uint32 -> c11: uint32 -> c12: uint32 -> c13: uint32 ->
-  c14: uint32 -> c15: uint32
-  -> o: lbuffer uint64 (size 4) ->
+  c14: uint32 -> c15: uint32 -> o: lbuffer uint64 (size 4) ->
   Stack unit
-    (requires fun h -> live h o)
-    (ensures fun h0 _ h1 -> modifies (loc o) h0 h1 /\ as_nat P256 h1 o == (v c14 + v c15 * pow2 32 + v c9 * pow2 (3 * 32) + v c10 * pow2 (4 * 32) + v c11 * pow2 (5 * 32) + v c13 * pow2 (7 * 32)) % prime256)
+  (requires fun h -> live h o)
+  (ensures fun h0 _ h1 -> modifies (loc o) h0 h1 /\ as_nat P256 h1 o == (v c14 + v c15 * pow2 32 + v c9 * pow2 (3 * 32) + v c10 * pow2 (4 * 32) + v c11 * pow2 (5 * 32) + v c13 * pow2 (7 * 32)) % prime256)
 
 let upl_eig_buffer c9 c10 c11 c12 c13 c14 c15 o =
   assert_norm (pow2 (1 * 32) * pow2 (2 * 32) = pow2 (3 * 32));
@@ -327,95 +343,91 @@ let upl_eig_buffer c9 c10 c11 c12 c13 c14 c15 o =
   assert_norm (pow2 (3 * 32) * pow2 (2 * 32) = pow2 (5 * 32));
   assert_norm (pow2 (4 * 32) * pow2 (2 * 32) = pow2 (6 * 32));
   assert_norm (pow2 (5 * 32) * pow2 (2 * 32) = pow2 (7 * 32));
-    let b0 = store_high_low_u c15 c14 in
-    let b1 = store_high_low_u c9 (u32 0) in
-    let b2 = store_high_low_u c11 c10 in
-    let b3 = store_high_low_u c13 (u32 0) in
-    load_buffer b0 b1 b2 b3 o;
-    reduction_prime_2prime #P256 o o
+  
+  let b0 = store_high_low_u c15 c14 in
+  let b1 = store_high_low_u c9 (u32 0) in
+  let b2 = store_high_low_u c11 c10 in
+  let b3 = store_high_low_u c13 (u32 0) in
+  
+  load_buffer b0 b1 b2 b3 o;
+  reduction_prime_2prime #P256 o o
 
 
 inline_for_extraction noextract
-val solinas_reduction_upload: c0: uint32 -> c1: uint32 -> c2: uint32 -> c3: uint32 -> c4: uint32 -> c5: uint32 -> c6: uint32 -> c7: uint32 -> c8: uint32 -> c9: uint32 -> c10: uint32 -> c11: uint32 -> c12: uint32 -> c13: uint32 -> c14: uint32 -> c15: uint32 -> tempBuffer: lbuffer uint64 (size 36) ->
+val solinas_reduction_upload: c0: uint32 -> c1: uint32 -> c2: uint32 -> c3: uint32 -> c4: uint32 -> c5: uint32 -> c6: uint32 
+  -> c7: uint32 -> c8: uint32 -> c9: uint32 -> c10: uint32 -> c11: uint32 -> c12: uint32 -> c13: uint32 -> c14: uint32 
+  -> c15: uint32 -> tempBuffer: lbuffer uint64 (size 36) ->
   Stack unit
-    (requires fun h -> live h tempBuffer)
-    (ensures fun h0 _ h1 -> modifies1 tempBuffer h0 h1 /\
-        (
-          let t0 = as_nat P256 h1 (gsub tempBuffer (size 0) (size 4)) in
-          let t1 = as_nat P256 h1 (gsub tempBuffer (size 4) (size 4)) in
-          let t2 = as_nat P256 h1 (gsub tempBuffer (size 8) (size 4)) in
-          let t3 = as_nat P256 h1 (gsub tempBuffer (size 12) (size 4)) in
-          let t4 = as_nat P256 h1 (gsub tempBuffer (size 16) (size 4)) in
-          let t5 = as_nat P256 h1 (gsub tempBuffer (size 20) (size 4)) in
-          let t6 = as_nat P256 h1 (gsub tempBuffer (size 24) (size 4)) in
-          let t7 = as_nat P256 h1 (gsub tempBuffer (size 28) (size 4)) in
-          let t8 = as_nat P256 h1 (gsub tempBuffer (size 32) (size 4)) in
-          t0 == (v c0 + v c1 * pow2 (1 * 32) + v c2 * pow2 (2 * 32) + v c3 * pow2 (3 * 32) + v c4 * pow2 (4 * 32) + v c5 * pow2 (5 * 32) + v  c6 * pow2 (6 * 32) +  v c7 * pow2 (7 * 32)) % prime /\
-          t1 == (v c11 * pow2 (3 * 32) + v c12 * pow2 (4 * 32) + v c13 * pow2 (5 * 32) +
-           v c14 * pow2 (6 * 32) + v c15 * pow2 (7 * 32)) % prime /\
-          t2 == (v c12 * pow2 (3 * 32) + v c13 * pow2 (4 * 32) +  v c14 * pow2 (5 * 32) + v c15 * pow2 (6 * 32)) % prime  /\
-          t3 == (v c8 + v c9 * pow2 32 + v c10 * pow2 (2 * 32) + v c14 * pow2 (6 * 32) + v c15 * pow2 (7 * 32)) % prime /\
-          t4 == (v c9 + v c10 * pow2 32 + v c11 * pow2 (2 * 32) + v c13 * pow2 (3 * 32) + v c14 * pow2 (4 * 32) + v c15 * pow2 (5 * 32) + v c13 * pow2 (6 * 32) + v c8 * pow2 (7 * 32)) % prime /\
-          t5 == (v c11 + v c12 * pow2 32 + v c13 * pow2 (2 * 32) + v c8 * pow2 (6 * 32) + v c10 * pow2 (7 * 32)) % prime /\
-          t6 == (v c12 + v c13 * pow2 32 + v c14 * pow2 (2 * 32) + v c15 * pow2 (3 * 32) + v c9 * pow2 (6 * 32) + v c11 * pow2 (7 * 32)) % prime /\
-          t7 == (v c13 + v c14 * pow2 32 + v c15 * pow2 (2 * 32) +  v c8 * pow2 (3 * 32) +  v c9 * pow2 (4 * 32) + v c10 * pow2 (5 * 32) + v c12 * pow2 (7 * 32)) % prime /\
-          t8 == (v c14 + v c15 * pow2 32 + v c9 * pow2 (3 * 32) +  v c10 * pow2 (4 * 32) + v c11 * pow2 (5 * 32) + v c13 * pow2 (7 * 32)) % prime
-    ))
+  (requires fun h -> live h tempBuffer)
+  (ensures fun h0 _ h1 -> modifies1 tempBuffer h0 h1 /\ (
+    let t0 = as_nat P256 h1 (gsub tempBuffer (size 0) (size 4)) in
+    let t1 = as_nat P256 h1 (gsub tempBuffer (size 4) (size 4)) in
+    let t2 = as_nat P256 h1 (gsub tempBuffer (size 8) (size 4)) in
+    let t3 = as_nat P256 h1 (gsub tempBuffer (size 12) (size 4)) in
+    let t4 = as_nat P256 h1 (gsub tempBuffer (size 16) (size 4)) in
+    let t5 = as_nat P256 h1 (gsub tempBuffer (size 20) (size 4)) in
+    let t6 = as_nat P256 h1 (gsub tempBuffer (size 24) (size 4)) in
+    let t7 = as_nat P256 h1 (gsub tempBuffer (size 28) (size 4)) in
+    let t8 = as_nat P256 h1 (gsub tempBuffer (size 32) (size 4)) in
+    
+    t0 == (v c0 + v c1 * pow2 (1 * 32) + v c2 * pow2 (2 * 32) + v c3 * pow2 (3 * 32) + v c4 * pow2 (4 * 32) + v c5 * pow2 (5 * 32) + v  c6 * pow2 (6 * 32) +  v c7 * pow2 (7 * 32)) % prime /\
+    t1 == (v c11 * pow2 (3 * 32) + v c12 * pow2 (4 * 32) + v c13 * pow2 (5 * 32) + v c14 * pow2 (6 * 32) + v c15 * pow2 (7 * 32)) % prime /\
+    t2 == (v c12 * pow2 (3 * 32) + v c13 * pow2 (4 * 32) +  v c14 * pow2 (5 * 32) + v c15 * pow2 (6 * 32)) % prime  /\
+    t3 == (v c8 + v c9 * pow2 32 + v c10 * pow2 (2 * 32) + v c14 * pow2 (6 * 32) + v c15 * pow2 (7 * 32)) % prime /\
+    t4 == (v c9 + v c10 * pow2 32 + v c11 * pow2 (2 * 32) + v c13 * pow2 (3 * 32) + v c14 * pow2 (4 * 32) + v c15 * pow2 (5 * 32) + v c13 * pow2 (6 * 32) + v c8 * pow2 (7 * 32)) % prime /\
+    t5 == (v c11 + v c12 * pow2 32 + v c13 * pow2 (2 * 32) + v c8 * pow2 (6 * 32) + v c10 * pow2 (7 * 32)) % prime /\
+    t6 == (v c12 + v c13 * pow2 32 + v c14 * pow2 (2 * 32) + v c15 * pow2 (3 * 32) + v c9 * pow2 (6 * 32) + v c11 * pow2 (7 * 32)) % prime /\
+    t7 == (v c13 + v c14 * pow2 32 + v c15 * pow2 (2 * 32) +  v c8 * pow2 (3 * 32) +  v c9 * pow2 (4 * 32) + v c10 * pow2 (5 * 32) + v c12 * pow2 (7 * 32)) % prime /\
+    t8 == (v c14 + v c15 * pow2 32 + v c9 * pow2 (3 * 32) +  v c10 * pow2 (4 * 32) + v c11 * pow2 (5 * 32) + v c13 * pow2 (7 * 32)) % prime))
 
 
 let solinas_reduction_upload c0 c1 c2 c3 c4 c5 c6 c7 c8 c9 c10 c11 c12 c13 c14 c15 tempBuffer =
-    let t0 = sub tempBuffer (size 0) (size 4) in
-    let t1 = sub tempBuffer (size 4) (size 4) in
-    let t2 = sub tempBuffer (size 8) (size 4) in
-    let t3 = sub tempBuffer (size 12) (size 4) in
-    let t4 = sub tempBuffer (size 16) (size 4) in
-    let t5 = sub tempBuffer (size 20) (size 4) in
-    let t6 = sub tempBuffer (size 24) (size 4) in
-    let t7 = sub tempBuffer (size 28) (size 4) in
-    let t8 = sub tempBuffer (size 32) (size 4) in
-    upl_zer_buffer c0 c1 c2 c3 c4 c5 c6 c7 t0;
-    upl_fir_buffer c11 c12 c13 c14 c15 t1;
-    upl_sec_buffer c12 c13 c14 c15 t2;
-    upl_thi_buffer c8 c9 c10 c14 c15  t3;
-    upl_for_buffer c8 c9 c10 c11 c13 c14 c15 t4;
-    upl_fif_buffer c8 c10 c11 c12 c13 t5;
-    upl_six_buffer c9 c11 c12 c13 c14 c15 t6;
-    upl_sev_buffer c8 c9 c10 c12 c13 c14 c15 t7;
-    upl_eig_buffer c9 c10 c11 c12 c13 c14 c15 t8
+  let t0 = sub tempBuffer (size 0) (size 4) in
+  let t1 = sub tempBuffer (size 4) (size 4) in
+  let t2 = sub tempBuffer (size 8) (size 4) in
+  let t3 = sub tempBuffer (size 12) (size 4) in
+  let t4 = sub tempBuffer (size 16) (size 4) in
+  let t5 = sub tempBuffer (size 20) (size 4) in
+  let t6 = sub tempBuffer (size 24) (size 4) in
+  let t7 = sub tempBuffer (size 28) (size 4) in
+  let t8 = sub tempBuffer (size 32) (size 4) in
+  
+  upl_zer_buffer c0 c1 c2 c3 c4 c5 c6 c7 t0;
+  upl_fir_buffer c11 c12 c13 c14 c15 t1;
+  upl_sec_buffer c12 c13 c14 c15 t2;
+  upl_thi_buffer c8 c9 c10 c14 c15  t3;
+  upl_for_buffer c8 c9 c10 c11 c13 c14 c15 t4;
+  upl_fif_buffer c8 c10 c11 c12 c13 t5;
+  upl_six_buffer c9 c11 c12 c13 c14 c15 t6;
+  upl_sev_buffer c8 c9 c10 c12 c13 c14 c15 t7;
+  upl_eig_buffer c9 c10 c11 c12 c13 c14 c15 t8
 
 
 inline_for_extraction noextract
-val solinas_reduction_operations: tempBuffer: lbuffer uint64 (size 36) ->  o: lbuffer uint64 (size 4) ->
+val solinas_reduction_operations: tempBuffer: lbuffer uint64 (size 36) -> o: lbuffer uint64 (size 4) ->
   Stack unit
-    (requires fun h -> live h o /\ live h tempBuffer /\ disjoint tempBuffer o /\
-      (
-          let t0 = as_nat P256 h (gsub tempBuffer (size 0) (size 4)) in
-          let t1 = as_nat P256 h (gsub tempBuffer (size 4) (size 4)) in
-          let t2 = as_nat P256 h (gsub tempBuffer (size 8) (size 4)) in
-          let t3 = as_nat P256 h (gsub tempBuffer (size 12) (size 4)) in
-          let t4 = as_nat P256 h (gsub tempBuffer (size 16) (size 4)) in
-          let t5 = as_nat P256 h (gsub tempBuffer (size 20) (size 4)) in
-          let t6 = as_nat P256 h (gsub tempBuffer (size 24) (size 4)) in
-          let t7 = as_nat P256 h (gsub tempBuffer (size 28) (size 4)) in
-          let t8 = as_nat P256 h (gsub tempBuffer (size 32) (size 4)) in
-          t0 < prime /\ t1 < prime /\ t2 < prime /\ t3 < prime /\ t4 < prime /\
-          t5 < prime /\ t6 < prime /\ t7 < prime /\ t8 < prime
-      )
-    )
-    (ensures fun h0 _ h1 -> modifies2 tempBuffer o h0 h1 /\
-       (
-          let t0 = as_nat P256 h0 (gsub tempBuffer (size 0) (size 4)) in
-          let t1 = as_nat P256 h0 (gsub tempBuffer (size 4) (size 4)) in
-          let t2 = as_nat P256 h0 (gsub tempBuffer (size 8) (size 4)) in
-          let t3 = as_nat P256 h0 (gsub tempBuffer (size 12) (size 4)) in
-          let t4 = as_nat P256 h0 (gsub tempBuffer (size 16) (size 4)) in
-          let t5 = as_nat P256 h0 (gsub tempBuffer (size 20) (size 4)) in
-          let t6 = as_nat P256 h0 (gsub tempBuffer (size 24) (size 4)) in
-          let t7 = as_nat P256 h0 (gsub tempBuffer (size 28) (size 4)) in
-          let t8 = as_nat P256 h0 (gsub tempBuffer (size 32) (size 4)) in
-          as_nat P256 h1 o == (t0 + 2 * t1 + 2 * t2  + t3 + t4 - t5  - t6 - t7 - t8) % prime
-    )
-  )
+  (requires fun h -> live h o /\ live h tempBuffer /\ disjoint tempBuffer o /\ (
+    let t0 = as_nat P256 h (gsub tempBuffer (size 0) (size 4)) in
+    let t1 = as_nat P256 h (gsub tempBuffer (size 4) (size 4)) in
+    let t2 = as_nat P256 h (gsub tempBuffer (size 8) (size 4)) in
+    let t3 = as_nat P256 h (gsub tempBuffer (size 12) (size 4)) in
+    let t4 = as_nat P256 h (gsub tempBuffer (size 16) (size 4)) in
+    let t5 = as_nat P256 h (gsub tempBuffer (size 20) (size 4)) in
+    let t6 = as_nat P256 h (gsub tempBuffer (size 24) (size 4)) in
+    let t7 = as_nat P256 h (gsub tempBuffer (size 28) (size 4)) in
+    let t8 = as_nat P256 h (gsub tempBuffer (size 32) (size 4)) in
+    t0 < prime /\ t1 < prime /\ t2 < prime /\ t3 < prime /\ t4 < prime /\ t5 < prime /\ t6 < prime /\ t7 < prime /\ t8 < prime))
+  (ensures fun h0 _ h1 -> modifies2 tempBuffer o h0 h1 /\ (
+    let t0 = as_nat P256 h0 (gsub tempBuffer (size 0) (size 4)) in
+    let t1 = as_nat P256 h0 (gsub tempBuffer (size 4) (size 4)) in
+    let t2 = as_nat P256 h0 (gsub tempBuffer (size 8) (size 4)) in
+    let t3 = as_nat P256 h0 (gsub tempBuffer (size 12) (size 4)) in
+    let t4 = as_nat P256 h0 (gsub tempBuffer (size 16) (size 4)) in
+    let t5 = as_nat P256 h0 (gsub tempBuffer (size 20) (size 4)) in
+    let t6 = as_nat P256 h0 (gsub tempBuffer (size 24) (size 4)) in
+    let t7 = as_nat P256 h0 (gsub tempBuffer (size 28) (size 4)) in
+    let t8 = as_nat P256 h0 (gsub tempBuffer (size 32) (size 4)) in
+    as_nat P256 h1 o == (t0 + 2 * t1 + 2 * t2  + t3 + t4 - t5  - t6 - t7 - t8) % prime))
 
 let solinas_reduction_operations tempBuffer o =
     let h0 = ST.get() in
@@ -472,7 +484,7 @@ val lemma_opened: i:Lib.Sequence.lseq uint64 8 -> Lemma
    let c14 = get_low_part  i7 in
    let c15 = get_high_part i7 in
 
-   felem_seq_as_nat_8 i =
+   lseq_as_nat i =
      v c0  * pow2 (0 * 32) +
      v c1  * pow2 (1 * 32) +
      v c2  * pow2 (2 * 32) +
@@ -490,7 +502,32 @@ val lemma_opened: i:Lib.Sequence.lseq uint64 8 -> Lemma
      v c14 * pow2 (14 * 32) +
      v c15 * pow2 (15 * 32))
 
-#push-options "--z3rlimit 400"
+#push-options "--z3rlimit 400 --fuel 1"
+
+val lemma_lseq_8_as_definition: i: Lib.Sequence.lseq uint64 8 -> Lemma (
+  let open Lib.Sequence in 
+  let i0 = index i 0 in
+  let i1 = index i 1 in
+  let i2 = index i 2 in
+  let i3 = index i 3 in
+  let i4 = index i 4 in
+  let i5 = index i 5 in
+  let i6 = index i 6 in
+  let i7 = index i 7 in 
+  lseq_as_nat i == v i0 * pow2 (0 * 64) + v i1 * pow2 (1 * 64) + v i2 * pow2 (2 * 64) + v i3 * pow2 (3 * 64) + v i4 * pow2 (4 * 64) + v i5 * pow2 (5 * 64) + v i6 * pow2 (6 * 64) + v i7 * pow2 (7 * 64))
+
+let lemma_lseq_8_as_definition i = 
+  lseq_as_nat_definiton i 0;
+  lseq_as_nat_definiton i 1;
+  lseq_as_nat_definiton i 2;
+  lseq_as_nat_definiton i 3;
+  
+  lseq_as_nat_definiton i 4;
+  lseq_as_nat_definiton i 5;
+  lseq_as_nat_definiton i 6;
+  lseq_as_nat_definiton i 7
+
+#pop-options
 
 let lemma_opened i =
   let open Lib.Sequence in
@@ -609,8 +646,8 @@ let lemma_opened i =
   };
 
   calc (==) {
-    felem_seq_as_nat_8 i;
-    == { }
+    lseq_as_nat i;
+    == { lemma_lseq_8_as_definition i }
     v i0 * pow2 (0 * 64) +
     v i1 * pow2 (1 * 64) +
     v i2 * pow2 (2 * 64) +
@@ -651,8 +688,8 @@ let lemma_opened i =
 val solinas_reduction_impl_p256: i: lbuffer uint64 (getCoordinateLenU64 P256 *. 2ul) 
   -> o: lbuffer uint64 (getCoordinateLenU64 P256) -> 
   Stack unit
-    (requires fun h -> live h i /\ live h o /\ disjoint i o)
-    (ensures fun h0 _ h1 -> modifies1 o h0 h1 /\ wide_as_nat P256 h0 i % (getPrime P256) == as_nat P256 h1 o)
+  (requires fun h -> live h i /\ live h o /\ disjoint i o)
+  (ensures fun h0 _ h1 -> modifies1 o h0 h1 /\ wide_as_nat P256 h0 i % (getPrime P256) == as_nat P256 h1 o)
 
 
 let solinas_reduction_impl_p256 i o =
@@ -706,7 +743,7 @@ let solinas_reduction_impl_p256 i o =
 
     solinas_reduction_mod (v c0) (v c1) (v c2) (v c3) (v c4) (v c5) (v c6) (v c7) (v c8) (v c9) (v c10) (v c11) (v c12) (v c13) (v c14) (v c15) (as_nat P256 h1 t0) (as_nat P256 h1 t1) (as_nat P256 h1 t2) (as_nat P256 h1 t3) (as_nat P256 h1 t4) (as_nat P256 h1 t5) (as_nat P256 h1 t6) (as_nat P256 h1 t7) (as_nat P256 h1 t8) (as_nat P256 h2 o);
 
-  modulo_lemma (as_nat P256 h2 o) prime;
+    modulo_lemma (as_nat P256 h2 o) prime;
   pop_frame()
 
 
